FTLR EInit: WIP preparation structure of the proof

theories/ftlr/EInit.v
@@ -3,7 +3,7 @@ From iris.program_logic Require Import weakestpre adequacy lifting.
 From stdpp Require Import base.
 From cap_machine Require Export logrel.
 From cap_machine.ftlr Require Import ftlr_base.
-From cap_machine.rules Require Import rules_Jmp.
+From cap_machine.rules Require Import rules_EInit.
 
 Section fundamental.
   Context {Σ:gFunctors} {ceriseg:ceriseG Σ} {sealsg: sealStoreG Σ}
@@ -16,88 +16,197 @@ Section fundamental.
   Implicit Types lw : (leibnizO LWord).
   Implicit Types interp : (D).
 
+  Local Hint Resolve finz_seq_between_NoDup list_remove_elem_NoDup : core.
+
+  (** Predicate that defines when the contents of a register can be swept;
+      i.e. when the register contains a capability with at least R permissions... *)
+  Definition reg_allows_einit
+    (lregs : LReg) (lmem : LMem) (r : RegName)
+    (b e a : Addr) (v : Version)
+    (b' e' a' : Addr) (v' : Version):=
+    lregs !! r = Some (LCap RX b e a v)
+    ∧ lmem !! (a,v) = Some (LCap RW b' e' a' v').
+
+  (* TODO move stdpp_extra *)
+  Fixpoint list_remove_elem_list `{A : Type} `{EqDecision A} (la' la : list A) : list A :=
+    match la' with
+    | [] => la
+    | h::t => list_remove_elem h (list_remove_elem_list t la)
+    end.
+
+  Definition code_addresses (a_pc : Addr) (code_la : list Addr)
+    := (list_remove_elem a_pc code_la).
+
+  Definition allow_einit_mask_code
+    (a_pc : Addr) (v_pc : Version)
+    (code_la : list Addr) (code_v : Version)
+    : coPset :=
+    let pc_mask := (⊤ ∖ ↑logN.@(a_pc, v_pc)) in
+    compute_mask_region pc_mask (code_addresses a_pc code_la) code_v.
+
+  Definition data_addresses (a_pc : Addr) (code_la data_la : list Addr)
+    := (list_remove_elem_list (a_pc::code_la) data_la).
+
+  Definition allow_einit_mask_data
+    (a_pc : Addr) (v_pc : Version)
+    (code_la : list Addr) (code_v : Version)
+    (data_la : list Addr) (data_v : Version)
+    : coPset :=
+    let code_mask := allow_einit_mask_code a_pc v_pc code_la code_v in
+    compute_mask_region code_mask (data_addresses a_pc code_la data_la) data_v.
+
+  (* Lemma allow_einit_mask_remove_nodup *)
+  (*   (a_pc : Addr) (v_pc : Version) (code_la data_la : list Addr) (v : Version) : *)
+  (*   NoDup code_la -> *)
+  (*   NoDup data_la -> *)
+  (*   allow_sweep_mask a_pc v_pc (list_remove_elem a_pc la) v = *)
+  (*   allow_sweep_mask a_pc v_pc la v. *)
+  (* Proof. *)
+  (*   intros HNoDup. *)
+  (*   by rewrite /allow_sweep_mask list_remove_elem_idem. *)
+  (* Qed. *)
+
+  (* this will help us close the invariant again... *)
+  (* it states which properties are enforced on all the lws *)
+
+
+  Definition region_open_resources
+    (a_pc : Addr) (v_pc : Version)
+    (code_la : list Addr) (code_v : Version)
+    (code_lws : list LWord) (code_Ps : list D)
+    (data_la : list Addr) (data_v : Version)
+    (data_lws : list LWord) (data_Ps : list D)
+    (has_later : bool)
+    : iProp Σ :=
+
+    let E := ⊤ ∖ ↑logN.@(a_pc, v_pc) in
+    let E1 := allow_einit_mask_code a_pc v_pc code_la code_v in
+    let E2 := allow_einit_mask_data a_pc v_pc code_la code_v data_la data_v in
+
+    ([∗ list] lw;Pw ∈ code_lws;code_Ps, (if has_later then ▷ (Pw : D) lw else (Pw : D) lw))
+    ∗ ([∗ list] lw;Pw ∈ data_lws;data_Ps, (if has_later then ▷▷ (Pw : D) lw else (Pw : D) lw))
+
+    ∗ ( ⌜ Persistent ([∗ list] lw;Pw ∈ code_lws;code_Ps, (Pw : D) lw) ⌝ ) (* All properties P are persistent *)
+    ∗ ( ⌜ Persistent ([∗ list] lw;Pw ∈ data_lws;data_Ps, (Pw : D) lw) ⌝ ) (* All properties P are persistent *)
+
+    ∗ ( if has_later
+        then ([∗ list] Pa ∈ code_Ps, read_cond Pa interp)
+             ∗ ([∗ list] Pa ∈ data_Ps, ▷ read_cond Pa interp)
+               (* the read cond holds *)
+        else ([∗ list] Pa ∈ code_Ps, (□ ∀ (lw : LWord), (Pa : D) lw -∗ interp lw))
+               ∗ ([∗ list] Pa ∈ data_Ps, (□ ∀ (lw : LWord), (Pa : D) lw -∗ interp lw))
+      )%I
+
+    ∗ (▷▷ ([∗ list] a_Pa ∈ zip data_la code_Ps, (interp_ref_inv a_Pa.1 data_v a_Pa.2)) ={E2, E1 }=∗ True)
+    ∗ (▷ ([∗ list] a_Pa ∈ zip code_la data_Ps, (interp_ref_inv a_Pa.1 code_v a_Pa.2)) ={E1, E }=∗ True).
+
+  Definition einit_mask_cond
+    (lregs : LReg) (lmem : LMem)
+    (src : RegName) (b_src e_src a_src : Addr) (v_src : Version)
+    (b' e' a' : Addr) (v' : Version)
+    (a_pc : Addr) (v_pc : Version) :=
+    (* TODO it misses something here: we need conditions over a_pc and b' e' *)
+    decide (reg_allows_einit lregs lmem src b_src e_src a_src v_src b' e' a' v'
+            /\ (src = PC \/ a_pc ∉ (finz.seq_between b_src e_src))
+      ).
+
+  (* Description of what the resources are supposed to look like after opening the region *)
+  (*    if we need to, but before closing the region up again*)
+
+  Definition allow_einit_res
+    (lregs : LReg) (lmem : LMem)
+    (src : RegName)
+    (a_pc : Addr) (v_pc : Version)
+    (b_code e_code a_code : Addr) (v_code : Version) (code_Ps : list D)
+    (b_data e_data a_data : Addr) (v_data : Version) (data_Ps : list D)
+    :=
+
+    let code_la  := code_addresses a_pc (finz.seq_between b_code e_code) in
+    let data_la  := data_addresses a_pc code_la (finz.seq_between b_data e_data) in
+    let E   := ⊤ ∖ ↑logN.@(a_pc, v_pc) in
+    let E1 := allow_einit_mask_code a_pc v_pc code_la v_code in
+    let E2 := allow_einit_mask_data a_pc v_pc code_la v_code data_la v_data in
+
+    (⌜read_reg_inr lregs src RX b_code e_code a_code v_code⌝ ∗
+     ⌜allows_einit lregs lmem src⌝ ∗
+     if einit_mask_cond lregs lmem
+          src b_code e_code a_code v_code
+          b_data e_data a_data v_data
+          a_pc v_pc
+     then
+      (|={E, E2}=> (* we open this invariant with all the points-tos from b to e *)
+         ∃ (code_lws : list LWord) (data_lws : list LWord),
+         ⌜ length code_lws = length code_la ⌝
+         ∗ ⌜ length data_lws = length data_la ⌝
+         ∗ ([∗ map] la↦lw ∈ (logical_region_map code_la code_lws v_code), la ↦ₐ lw) (* here you get all the points-tos *)
+         ∗ ([∗ map] la↦lw ∈ (logical_region_map data_la data_lws v_data), la ↦ₐ lw)
+         ∗ region_open_resources a_pc v_pc
+             code_la v_code code_lws code_Ps
+             data_la v_data data_lws data_Ps
+             true)%I
+     else True)%I.
+
+  (* this does not yet open the invariant *)
+  Lemma create_einit_res
+    (lregs : LReg) (lmem : LMem)
+    (src : RegName)
+    (p_pc : Perm) (b_pc e_pc a_pc : Addr) (v_pc : Version)
+    (b_code e_code a_code : Addr) (v_code : Version)
+    (b_data e_data a_data : Addr) (v_data : Version) :
+
+    let code_la  := code_addresses a_pc (finz.seq_between b_code e_code) in
+    let data_la  := data_addresses a_pc code_la (finz.seq_between b_data e_data) in
+
+    read_reg_inr (<[PC:=LCap p_pc b_pc e_pc a_pc v_pc]> lregs) src RX b_code e_code a_code v_code
+    -> a_pc ∈ finz.seq_between b_pc e_pc
+    → (∀ (r : RegName) lw, ⌜r ≠ PC⌝ → ⌜lregs !! r = Some lw⌝ → (fixpoint interp1) lw)
+    -∗ interp (LCap p_pc b_pc e_pc a_pc v_pc)
+    -∗ (∃ (code_Ps : list D) (data_Ps  : list D),
+           ⌜ length code_la = length code_Ps ⌝
+           ∗ ⌜length data_la = length data_Ps ⌝
+           ∗ allow_einit_res
+               (<[PC:=LCap p_pc b_pc e_pc a_pc v_pc]> lregs) lmem src
+               a_pc v_pc
+               b_code e_code a_code v_code code_Ps
+               b_data e_data a_data v_data data_Ps
+       ).
+  Proof.
+  Admitted.
+
+  Definition allow_einit_mem
+    (lmem : LMem) (lregs : LReg) (src : RegName)
+    (a_pc : Addr) (v_pc : Version) (lw_pc : LWord)
+
+    (b_code e_code a_code : Addr) (v_code : Version) (code_Ps : list D)
+    (b_data e_data a_data : Addr) (v_data : Version) (data_Ps : list D)
+
+    (has_later : bool) :=
+
+    let code_la  := code_addresses a_pc (finz.seq_between b_code e_code) in
+    let data_la  := data_addresses a_pc code_la (finz.seq_between b_data e_data) in
+
+    (⌜read_reg_inr lregs src RX b_code e_code a_code v_code⌝ ∗
+     if einit_mask_cond lregs lmem
+          src b_code e_code a_code v_code
+          b_data e_data a_data v_data
+          a_pc v_pc
+     then (∃ (code_lws : list LWord) (data_lws : list LWord),
+           ⌜ length code_la = length code_lws ⌝
+           ∗ ⌜length data_la = length data_lws ⌝
+           ∗ ⌜lmem = <[(a_pc, v_pc):=lw_pc]>
+                       (logical_region_map code_la code_lws v_code
+                          ∪ logical_region_map data_la data_lws v_data)⌝
+              ∗ region_open_resources a_pc v_pc
+                  code_la v_code code_lws code_Ps
+                  data_la v_data data_lws data_Ps
+                  has_later)
+     else ⌜lmem = <[(a_pc, v_pc):=lw_pc]> ∅⌝)%I.
+
   Lemma einit_case (lregs : leibnizO LReg)
     (p : Perm) (b e a : Addr) (v : Version)
     (lw : LWord) (r : RegName) (P : D):
     ftlr_instr lregs p b e a v lw (EInit r) P.
   Proof.
-  (*   intros Hp Hsome i Hbae Hi. *)
-  (*   iIntros "#IH #Hinv #Hinva #Hreg #Hread Hown Ha HP Hcls HPC Hmap". *)
-  (*   rewrite delete_insert_delete. *)
-  (*   destruct (reg_eq_dec PC r); simplify_map_eq. *)
-  (*   * iApply (wp_jmp_successPC with "[HPC Ha]"); eauto; first iFrame. *)
-  (*     iNext. iIntros "[HPC Ha] /=". *)
-  (*     (* reconstruct invariant *) *)
-  (*     iMod ("Hcls" with "[Ha HP]") as "_";[iExists lw;iFrame|]. *)
-  (*     iModIntro. *)
-  (*     iApply wp_pure_step_later; auto. *)
-  (*     (* reconstruct registers *) *)
-  (*     iNext. *)
-  (*     iDestruct ((big_sepM_delete _ _ PC) with "[HPC Hmap]") as "Hmap /="; *)
-  (*       [apply lookup_insert|rewrite delete_insert_delete;iFrame|]. simpl. *)
-  (*     (* apply IH *) *)
-  (*     iIntros "_". *)
-  (*     iApply ("IH" $! _ _ b e a with "[] [] [Hmap] [$Hown]"); eauto. *)
-  (*     { iPureIntro. apply Hsome. } *)
-  (*     destruct Hp as [-> | ->]; iFrame. *)
-  (*   * specialize Hsome with r as Hr. *)
-  (*     destruct Hr as [wsrc Hsomesrc]. *)
-  (*     iDestruct ((big_sepM_delete _ _ r) with "Hmap") as "[Hsrc Hmap]"; eauto. *)
-  (*     rewrite (lookup_delete_ne lregs PC r); eauto. *)
-  (*     iApply (wp_jmp_success with "[$HPC $Ha $Hsrc]"); eauto. *)
-  (*     iNext. iIntros "[HPC [Ha Hsrc]] /=". *)
-  (*     iApply wp_pure_step_later; auto. *)
-  (*     (* reconstruct regions *) *)
-  (*     iDestruct ((big_sepM_delete _ _ r) with "[Hsrc Hmap]") as "Hmap /="; *)
-  (*       [apply lookup_insert|rewrite delete_insert_delete;iFrame|]. *)
-  (*     rewrite -delete_insert_ne // insert_id; auto. *)
-
-  (*     iMod ("Hcls" with "[HP Ha]");[iExists lw;iFrame|iModIntro]. *)
-
-  (*    (* Needed because IH disallows non-capability values *) *)
-  (*     destruct wsrc as [ | [p' b' e' a' v' | ] | ]; cycle 1. *)
-  (*     { *)
-  (*       rewrite /updatePcPerm. *)
-  (*       (* Special case for E-values*) *)
-  (*       destruct (decide (p' = E)) as [-> | HneE]. *)
-  (*       - *)
-  (*         unshelve iDestruct ("Hreg" $! r _ _ Hsomesrc) as "HPCv"; auto. *)
-  (*         iClear "Hinv". *)
-  (*         rewrite fixpoint_interp1_eq; simpl. *)
-
-  (*         iDestruct (big_sepM_insert _ _ PC with "[$Hmap $HPC]") as "Hmap"; [apply lookup_delete|]. *)
-  (*         rewrite insert_delete_insert; auto. *)
-  (*         iDestruct ("HPCv" with "[$Hmap $Hown]") as "Hcont"; auto. *)
-  (*       - iAssert (PC ↦ᵣ LCap p' b' e' a' v')%I  with "[HPC]" as "HPC". *)
-  (*         { destruct p'; auto. congruence. } *)
-
-  (*         iDestruct (big_sepM_insert _ _ PC with "[$Hmap $HPC]") as "Hmap"; [apply lookup_delete|]. *)
-  (*         rewrite insert_delete_insert; auto. *)
-  (*         iNext; iIntros "_". *)
-  (*         iApply ("IH" $! (<[PC:=LCap p' b' e' a' v']> lregs) with "[%] [] [Hmap] [$Hown]"). *)
-  (*         { cbn. intros. by repeat (rewrite lookup_insert_is_Some'; right). } *)
-  (*         { iIntros (ri ? Hri Hvs). *)
-  (*           rewrite lookup_insert_ne in Hvs; auto. *)
-  (*           destruct (decide (ri = r)); simplify_map_eq. *)
-  (*           { rewrite Hsomesrc in Hvs; inversion Hvs; subst; clear Hvs. *)
-  (*             unshelve iSpecialize ("Hreg" $! r _ _ Hsomesrc); eauto. } *)
-  (*           { iApply "Hreg"; auto. } *)
-  (*         } *)
-  (*         { rewrite insert_insert. iApply "Hmap". } *)
-  (*         iModIntro. *)
-  (*         unshelve iSpecialize ("Hreg" $! r _ _ Hsomesrc); eauto. *)
-  (*     } *)
-
-  (*    (* Non-capability cases *) *)
-  (*     all: iNext; iIntros "_". *)
-  (*     all: rewrite /updatePcPerm; iApply (wp_bind (fill [SeqCtx])); *)
-  (*       iApply (wp_notCorrectPC with "HPC"); [intros HFalse; inversion HFalse; cbn in *; simplify_eq| ]. *)
-  (*     all: repeat iNext; iIntros "HPC /=". *)
-  (*     all: iApply wp_pure_step_later; auto. *)
-  (*     all: iNext; iIntros "_". *)
-  (*     all: iApply wp_value. *)
-  (*     all: iIntros; discriminate. *)
-  (* Qed. *)
-    Admitted.
+  Admitted.
 
 End fundamental.
